AltTraces.v
@@ -1,0 +1,119 @@
+Require Import List.
+Import ListNotations.
+
+Require Import Debruijn Derivations Occurrences FLSubformulas.
+Local Open Scope eqb_scope.
+Local Open Scope form.
+
+
+(** DEFINITION *)
+
+(** Finite Paths *)
+
+Definition FPathType := list sequent.
+
+Inductive preFPath : FPathType -> derivation -> Prop :=
+ | Lf s s' ls R: s = (oseq_forget s') -> preFPath [s] (ORule ls R s' []) 
+ | COne d t R ls s s': 
+                          preFPath t d -> s' = oseq_forget s -> preFPath (s'::t) (ORule ls R s [d])
+ | CLeft d d' R ls t s s': 
+                          preFPath t d -> s' = oseq_forget s -> preFPath (s'::t) (ORule ls R s [d;d'])
+ | CRight d d' R ls t s s': 
+                          preFPath t d -> s' = oseq_forget s -> preFPath (s'::t) (ORule ls R s [d';d]).
+
+Definition preFPathNode (t:FPathType)(d:derivation)(a:address) :=
+  match subderiv d a with
+  | None       => False
+  | Some d'  => preFPath t d'
+  end.
+
+Definition FPath (t:FPathType)(d:derivation)(a:address) : Prop := (Valid d) /\ (preFPathNode t d a). 
+
+(** FInite Traces *)
+
+Definition FTraceType := list (formula*sequent).
+
+Inductive preFTrace : FTraceType -> derivation -> Prop :=
+ | Leaf f s s' ls R: s = (oseq_forget s') -> InSeq f s -> preFTrace [(f,s)] (ORule ls R s' []) 
+ | ConsOne d t R ls s0 s s' f1 f2: 
+                          preFTrace ((f1,s0)::t) d -> s' = oseq_forget s 
+                          -> InSeq f2 s' -> In f1 (FL f2) 
+                          -> preFTrace ((f2,s')::(f1,s0)::t) (ORule ls R s [d])
+ | ConsLeft d d' t R ls s0 s s' f1 f2: 
+                          preFTrace ((f1,s0)::t) d -> s' = oseq_forget s 
+                          -> InSeq f2 s' -> In f1 (FL f2) 
+                          -> preFTrace ((f2,s')::(f1,s0)::t) (ORule ls R s [d;d'])
+ | ConsRight d d' t R ls s0 s s' f1 f2: 
+                          preFTrace ((f1,s0)::t) d -> s' = oseq_forget s 
+                          -> InSeq f2 s' -> In f1 (FL f2) 
+                          -> preFTrace ((f2,s')::(f1,s0)::t) (ORule ls R s [d';d])
+                        .
+
+Definition preFTraceNode (t:FTraceType)(d:derivation)(a:address) :=
+  match subderiv d a with
+  | None       => False
+  | Some d'  => preFTrace t d'
+  end.
+
+Definition FTrace (t:FTraceType)(d:derivation)(a:address) : Prop := (Valid d) /\ (preFTraceNode t d a). 
+
+
+(** Link between both*)
+
+Definition IsFTrace (t:FTraceType)(p:FPathType): Prop := map snd t = p. 
+
+
+(** Example *)
+
+Definition FTrace_example: FTraceType := 
+  [( ν (%0)⊕(%0), ⊦ [(ν (%0)⊕(%0))]);
+   (((ν (%0)⊕(%0)) ⊕ (ν (%0)⊕(%0))), ⊦ [((ν (%0)⊕(%0)) ⊕ (ν (%0)⊕(%0)))] );
+   (ν (%0)⊕(%0), ⊦ [ν (%0)⊕(%0)] )].
+
+Lemma FTrace_example_lemma : FTrace FTrace_example oderiv_example' [].
+Proof.
+  split;
+  repeat (constructor; simpl; intuition).
+Qed.
+
+(** Infinite Paths/Traces *)
+
+Definition PathType: Type := nat -> FPathType.
+
+Definition TraceType: Type := nat -> FTraceType.
+
+(** Link between both *)
+
+Definition IsTrace (T:TraceType)(P:PathType): Prop := forall n, map snd (T n) = P n. 
+
+(** Example *)
+
+Definition PathRepeat (t:FPathType) := (fun (n:nat) => t).
+
+Definition TraceRepeat (t:FTraceType) := (fun (n:nat) => t).
+
+Definition Trace_Example := TraceRepeat FTrace_example.
+
+
+
+
+
+
+
+(** PATH & TRACE VALIDITY *)
+
+Local Open Scope eqb_scope.
+
+(** Access to the last rule used in [d] (following address [a] in [d]) *)
+
+Definition last_trace_rule (d:derivation)(a:address) : option rule_kind :=
+  match subderiv d a with
+  | None => None
+  | Some d' => let '(ORule ls R s ld) := d' in match ld with 
+                                                                   | [] => Some R
+                                                                   | _ => None
+                                                                   end
+  end.
+
+(** Linking condition between Stream's elements *)
+
